add fizzBuzz libarary

examples/fizzBuzz/callFizzBuzz.c
@@ -3,6 +3,18 @@
 
 #include "FizzBuzz.h"
 
+#define MAX_N 100000U
+
+int fizzBuzz(uint32_t n) {
+    if (n == 0U || n > MAX_N) {
+        printf("n is out of range. (n: U32.t{ 0 < U32.v n /\\ U32.v n < 100000})\n");
+        return 1;
+    }
+    // val fizzBuzz : n: U32.t{ 0 < U32.v n /\ U32.v n < 100000} -> Stack C.exit_code (fun _ -> True) (fun _ _ _ -> True)
+    return fizzBuzzLib(n);
+}
+
 int main(int argc, char *argv[]) {
-    fizzBuzz();
+    int r = fizzBuzz(30U);
+    return r;
 }
